Finished Vector proofs

proof/DeclarativeTyping.v
@@ -17,7 +17,6 @@ Hint Resolve SubConv SubPi SubSigma SubLeft SubRight SubTrans : CCP.
 
 
 Definition ctx (n : nat) := @vec term n.
-Definition vnil := vnil term.
 
 Infix ":::" := vcons (at level 60, right associativity) : vec_scope.
 
@@ -30,7 +29,7 @@ Inductive wfd : forall n : nat, ctx n -> Prop :=
   | WfVar : forall n, forall G : ctx n, forall A s, typed n G A (sort s) -> wfd (S n) (A ::: G)
 with typed : forall n : nat, ctx n -> term -> term -> Prop :=
   | Var : forall n, forall G : ctx n, wfd n G -> 
-    forall i, forall p : i < n, typed n G (rel i) (lift i (nth p G))
+    forall i, forall p : i < n, typed n G (rel i) (lift i (nth i n p G))
     
   | Prod : forall n, forall G : ctx n, forall A B s_1 s_2, 
     typed n G A (sort s_1) -> typed (S n) (A ::: G) B (sort s_2) ->
@@ -73,7 +72,7 @@ with typed : forall n : nat, ctx n -> term -> term -> Prop :=
 
 
 Definition lift_ctx_rec (n k l : nat) (G : ctx l) :=
-  vmap (fun t => lift_rec n t k) G.
+  vmap l term term (fun t => lift_rec n t k) G.
 
 Definition lift_ctx (n l : nat) (G : ctx l) := lift_ctx_rec n 0 l G.
 
@@ -84,6 +83,8 @@ Hint Resolve Var Prod Abs SortT App LetIn Sum Pair LetTuple SubsetI Conv Subsum 
 
 Scheme typed_mut := Induction for typed Sort Prop
 with wfd_mut := Induction for wfd Sort Prop.
+
+Scheme typed_depind := Induction for typed Sort Prop.
 
 Lemma typed_wf : forall n, forall G : ctx n, forall t T, typed n G t T -> wfd n G.
 Proof.
@@ -108,33 +109,57 @@ Ltac eautoc := eauto with arith CCP.
 
 Require Import Lt.
 
-
+Set Implicit Arguments.
 Infix "+++" := vapp (right associativity, at level 60) : vector_scope.
-Check (vapp vnil vnil).
-Lemma weakening : forall n m, forall G : ctx n, forall G' : ctx m, forall U t T, 
-  typed (m + n) (vapp G' G) t T ->
-  wfd (m + S n) (vapp (lift_ctx 1 m G') (U ::: G)) -> 
-  typed (m + S n) (vapp (lift_ctx 1 m G') (U ::: G)) (lift_rec 1 t m)
+
+Lemma weakening : forall n m, forall G : ctx n, forall G' : ctx m, forall t T, 
+  typed (m + n) (vapp term m n G' G) t T ->
+  forall U,
+  wfd (m + S n) (vapp term m (S n) (lift_ctx 1 m G') (U ::: G)) -> 
+  typed (m + S n) (vapp term m (S n) (lift_ctx 1 m G') (U ::: G)) (lift_rec 1 t m)
   (lift_rec 1 T m).
 Proof.
-  intros n m G G' U t T Ht Hw. 
-  induction m.
+  intros n m.
+  intros G G' t T Ht.
+  induction Ht ; simpl ; intros.
+
+  elim (le_gt_dec m i) ; intros.
+  unfold lift.
+  rewrite simpl_lift_rec ; auto with arith.
   simpl.
-  simpl in Hw.
-  rewrite (eq_vnil G').
-  rewrite (eq_vnil G') in Ht.
-  rewrite (eq_vnil G') in Hw.
+  rewrite (cons_nth term n0 i G0 U).
+  pose Var.
+  unfold lift in t.
+
+
+inversion G0.
+
+  induction m ; simpl ; intros G G' U t T Ht Hw. 
+  rewrite (eq_vnil _ G').
+  rewrite (eq_vnil _ G') in Ht.
+  rewrite (eq_vnil _ G') in Hw.
   simpl in Ht, Hw.
   simpl.
-  induction Ht.
+  induction Ht using typed_depind.
+
   simpl.
   unfold lift.
-  rewrite simpl_lift_rec.
+  rewrite simpl_lift_rec ; auto with arith.
   simpl.
-  assert().
-  induction i ; simpl.
+  rewrite (cons_nth term n i G U).
+  pose Var.
+  unfold lift in t.
+  apply t ; auto.
+  
+  simpl ; simpl in IHHt1, IHHt2.
+  eapply Prod.
+  apply IHHt1; auto.
+  
+  
 
-  apply Var.
+  Lemma ctx_permut : forall n, forall U A, forall G : ctx n,
+  wfd (S n) (U ::: G) -> wfd (S n) (A ::: G) ->
+  
 
 
   apply Var.
